

**Autoregressive (AR)** \* AR always invertible

$\Phi_p(B)x_t = w_t$  where  $\Phi_p(B) = 1 - \phi_1 B - \phi_2 B^2 \dots$  or no solution

Causal condition:  $|\text{root to } \Phi_p(z)| > 1$  or  $\Phi_p(B)^{-1} = \Psi_\infty(B)$  for some  $\Psi$

• AR(1):  $|\phi_1| < 1$  • AR(2):  $|\phi_2| < 1$   $\phi_1 + \phi_2 < 1$   $\phi_2 - \phi_1 < 1$

AR(p) to MA( $\infty$ )

$\Phi_p(B)x_t = w_t \Rightarrow x_t = \Psi_\infty(B)w_t$  where  $\Psi_\infty(B) = 1 + \psi_1 B + \psi_2 B^2 \dots$

use  $\Phi_p(B) \cdot \Psi_\infty(B) = 1$  we can derive coefficients  $\psi_i$

$\psi_0 = 1$   $\psi_j = \phi_1 \psi_{j-1} + \phi_2 \psi_{j-2} + \dots$

\* MA always stationary and causal

Moving-average (MA)

$x_t = \Theta_q(B)w_t$  where  $\Theta_q(B) = 1 + \theta_1 B + \theta_2 B^2 \dots$  or no solution

Invertible condition:  $|\text{root to } \Theta_q(z)| > 1$  or  $\Theta_q(B)^{-1} = \Pi_\infty(B)$  for some  $\Pi$

• MA(1):  $|\theta_1| < 1$  • MA(2):  $|\theta_2| < 1$   $\theta_1 + \theta_2 < 1$   $\theta_2 - \theta_1 < 1$

MA(q) to AR( $\infty$ )

$x_t = \Theta_q(B)w_t \Rightarrow \Pi_\infty(B)x_t = w_t$  where  $\Pi_\infty(B) = 1 - \pi_1 B - \pi_2 B^2 \dots$

use  $\Theta_q(B) \cdot \Pi_\infty(B) = 1$  we can derive coefficients  $\pi_i$

$\pi_0 = -1$   $\pi_j = -\theta_1 \pi_{j-1} - \theta_2 \pi_{j-2} - \dots$

ARMA(p,q)

$\Phi_p(B)x_t = \Theta_q(B)w_t$  where  $\Phi_p(B) = 1 - \phi_1 B - \phi_2 B^2 \dots$   
 $\Theta_q(B) = 1 + \theta_1 B + \theta_2 B^2 \dots$

Causal condition:  $|\text{root to } \Phi_p(z)| > 1$

Invertible condition:  $|\text{root to } \Theta_q(z)| > 1$

Identifiability:  $\Phi_p(z) = 0$  and  $\Theta_q(z) = 0$  has no common roots

Causal ARMA(p,q) to MA( $\infty$ )

$\Phi_p(B)x_t = \Theta_q(B)w_t \Rightarrow x_t = \Psi_\infty(B)w_t$

use  $\Phi_p(B) \cdot \Psi_\infty(B) = \Theta_q(B)$  we can derive coefficients  $\psi_i$

$\psi_0 = 1$   $\psi_j = \theta_j + \phi_1 \psi_{j-1} + \phi_2 \psi_{j-2} + \dots$

Invertible ARMA(p,q) to AR( $\infty$ )

$\Phi_p(B)x_t = \Theta_q(B)w_t \Rightarrow \Pi_\infty(B)x_t = w_t$

use  $\Phi_p(B) \cdot \Pi_\infty(B) = \Theta_q(B)$  we can derive coefficients  $\pi_i$

$\pi_0 = -1$   $\pi_j = \theta_j - \phi_1 \pi_{j-1} - \phi_2 \pi_{j-2} - \dots$

ARIMA(p,d,q)

$\Phi_p(B)(1-B)^d x_t = \delta + \Theta_q(B)w_t$  where  $\delta = \mu(1 - \phi_1 - \phi_2 - \dots - \phi_p)$   
 ex:  $(1 - \phi_1 B - \phi_2 B^2)(1-B)^d x_t = (1 + \theta_1 B)w_t$  is ARIMA(2,1,1)  
 $p=2$   $d=1$   $q=1$

\* Proof

• AR(1)  $x_t - \phi_1 x_{t-1} = w_t$   
 mean  $E(x_t) = \sum_0^\infty \phi_i w_{t-i} = 0$   
 variance  $\gamma(0) = E(\sum_0^\infty \phi_i w_{t-i})^2 = \sigma_w^2 \sum_0^\infty \phi_i^2 = \frac{\sigma_w^2}{1 - \phi_1^2}$   
 covariance  $\gamma(h) = E(x_t x_{t+h}) = \sigma_w^2 \sum_0^\infty \phi_i \phi_i^{h+1} = \phi_1^h \sigma_w^2 \sum_0^\infty \phi_i^2 = \sigma_w^2 \frac{\phi_1^h}{1 - \phi_1^2}$   
 ACF  $\rho(h) = \frac{\gamma(h)}{\gamma(0)} = \phi_1^h$

• AR(2)  $x_t - \phi_1 x_{t-1} - \phi_2 x_{t-2} = w_t$   
 covariance  $\gamma(h) = E(x_t x_{t+h}) = \phi_1 \gamma(h-1) + \phi_2 \gamma(h-2)$   
 ACF  $\rho(1) = \frac{\phi_1}{1 - \phi_2}$   $\rho(2) = \frac{\phi_1^2}{1 - \phi_2} + \phi_2$   
 $\rho(h) = \phi_1 \rho(h-1) + \phi_2 \rho(h-2)$  for  $h \geq 3$

Derivation -  
 $E(x_t x_{t+h}) = \phi_1 E(x_{t-1} x_{t+h}) + \phi_2 E(x_{t-2} x_{t+h}) + E(w_t w_{t+h})$   
 divide by  $\gamma(0)$   
 $\gamma(h) = \phi_1 \gamma(h-1) + \phi_2 \gamma(h-2)$   
 use  $\rho(0) = 1$ ,  $\rho(1) = \rho(-1)$  get result

• AR(p) ACF  $\rho(h) = \phi_1 \rho(h-1) + \phi_2 \rho(h-2) + \dots$   
 $\phi_{hh} = \phi_h$  for  $h \leq p$ ,  $= 0$  for  $h > p$   
 $\phi_{hh} = \text{corr}(x_{t+h} - \hat{x}_{t+h}, x_t - \hat{x}_t)$   
 $\phi_{11} = \rho(1)$   $\phi_{pp} = \phi_p$  \* for any model AR, MA, ARMA

• MA(1)  $x_t = w_t + \theta w_{t-1}$  **trend of scatterplot = covariance**  
 mean  $E(x_t) = 0$   
 variance  $\gamma(0) = E(w_t^2 + 2\theta w_t w_{t-1} + \theta^2 w_{t-1}^2) = (1 + \theta^2) \sigma_w^2$   
 covariance  $\gamma(h) = E(w_t w_{t-h}) + \theta E(w_{t-1} w_{t-h}) + \theta E(w_t w_{t-h}) + \theta^2 E(w_{t-1} w_{t-h-1})$   
 $= (1 + \theta^2) \sigma_w^2$  for  $h=0$ ,  $\theta \sigma_w^2$  for  $h=\pm 1$ ,  $0$  for  $h=\pm 2, \pm 3, \dots$   
 ACF  $\rho(h) = \frac{\gamma(h)}{\gamma(0)} = 1$  for  $h=0$ ,  $\frac{\theta}{1+\theta^2}$  for  $h=\pm 1$ ,  $0$  for  $h=\pm 2, \pm 3, \dots$   
 PACF  $\phi_{hh} = (1-\theta)^h (1-\theta^2)^{-1} (1-\theta^{2(h+1)})^{-1}$  for  $h \geq 1$

• MA(2)  $x_t = w_t + \theta_1 w_{t-1} + \theta_2 w_{t-2}$   
 ACF  $\rho(1) = \frac{\theta_1(1+\theta_2)}{1+\theta_1^2+\theta_2^2}$   $\rho(2) = \frac{\theta_2}{1+\theta_1^2+\theta_2^2}$   $\rho(h) = 0$  for  $h \geq 2$

• MA(q) mean  $E(x_t) = \sum_0^q \theta_j E(w_{t-j}) = 0$   
 variance  $\gamma(0) = (1 + \theta_1^2 + \theta_2^2 + \dots + \theta_q^2) \sigma_w^2$   
 covariance  $\gamma(h) = \sigma_w^2 \sum_k^q \theta_k \theta_{k-h}$  for  $h=0 \dots \pm q$ ,  $0$  for  $h > q$   
 ACF  $\rho(h) = \frac{\gamma(h)}{\gamma(0)} = \frac{\sum_k^q \theta_k \theta_{k-h}}{(\sum_0^q \theta_j^2)}$  for  $h=0 \dots \pm q$ ,  $0$  for  $h > q$

• ARMA(1,1)  $x_t - \phi x_{t-1} = w_t + \theta w_{t-1}$   
 covariance  $\gamma(0) = \sigma_w^2 \frac{(1+\phi\theta + \theta^2)}{1-\phi^2}$   $\gamma(h) = \sigma_w^2 \frac{(1-\phi\theta)(\phi+\theta)}{1-\phi^2} \phi^{h-1}$  for  $h \geq 1$   
 ACF  $\rho(h) = \frac{\gamma(h)}{\gamma(0)} = \frac{(1-\phi\theta)(\phi+\theta)}{1+\phi\theta + \theta^2} \phi^{h-1}$  for  $h \geq 1$

ARIMA(p,d,q) x (P,D,Q)<sub>s</sub>  
 $\Phi_p(B) \cdot \Phi_p(B)^d \cdot (1-B)^d x_t = \delta + \Theta_q(B) \cdot \Theta_q(B)^d w_t$   
 ex:  $(1-0.5B)(1-B)^4 x_t = (1-0.3B)w_t$  is ARIMA(1,0,1) x (0,1,0)<sub>s</sub>  
 $p=1$   $s=4$   $d=1$   $q=1$

	PACF	zero	spike through lag p	cut off after lag p	tails off exp decay (damped or oscillation)	decay at lag p (direct or oscillation)	zero after lag 1
	ACF	zero	exp decay (direct or oscillation)	cut off after lag q	decay at lag q (direct or oscillation)	zero	
white noise	AR(p)	MA(q)	ARMA(p,q)	random walk			

	ACF	PCF
AR(P) <sub>s</sub>	tails off at lag k x s	cuts off after lag P x s
ARIMA(0) x (P, 0, 0) <sub>s</sub>		
MA(Q) <sub>s</sub>	cuts off at lag Q x s	tails off at lag k x s
ARIMA(0) x (0, 0, Q) <sub>s</sub>		
ARMA(P, Q) <sub>s</sub>	tails off at lag k x s	tails off at lag k x s
ARIMA(0) x (P, 0, Q) <sub>s</sub>		

Derivation:  
 $\gamma(h) = \text{Cov}(x_{t+h}, x_t) = E(x_{t+h} x_t)$   
 $= \phi E(x_{t+h-1} x_t) + E(w_{t+h} x_t) + \theta E(w_{t+h-1} x_t)$   
 $\downarrow$   
 $E(w_{t+h-1} \sum_0^q \psi_j w_{t-j})$   $E(w_{t+h-1} \sum_0^q \psi_j w_{t-j})$   
 $\begin{cases} \psi_0 \sigma_w^2 & h=0 \\ \psi_0 \sigma_w^2 & h=1 \\ 0 & h \geq 2 \end{cases}$   $\begin{cases} \psi_0 \sigma_w^2 & h=0 \\ 0 & h \geq 1 \end{cases}$   
 $\gamma(h) = \begin{cases} \phi \gamma(0) + \sigma_w^2 (1 + \phi\theta + \theta^2) & h=0 \\ \phi \gamma(0) + \sigma_w^2 \theta & h=1 \\ \phi \gamma(h-1) & h \geq 2 \end{cases} \Rightarrow \gamma(h) = \phi^{h-1} \gamma(1)$

Initial condition  $\begin{cases} \gamma(0) = \phi \gamma(0) + \sigma_w^2 (1 + \phi\theta + \theta^2) \\ \gamma(1) = \phi \gamma(0) + \sigma_w^2 \theta \end{cases}$   
 solve for  $\gamma(0)$ ,  $\gamma(1)$ , and get  $\gamma(h)$

weak station:  $E(x_t)$  doesn't depend on  $t$ , finite variance  
 auto covariance:  $\gamma(h) = \text{Cov}(x_t, x_{t+h})$

Model selection:  $\max R^2 \min \text{AIC, SSE}$   
 $\text{AIC} = \log \hat{\sigma}_k^2 + \frac{n+2k}{n}$   $\text{BIC} = \log \hat{\sigma}_k^2 + \frac{k \log n}{n}$  Linear model  
 $\text{AIC}_c = \log \hat{\sigma}_k^2 + \frac{n+k}{n-k-2}$   $\hat{\sigma}_k^2 = \text{SSE}(k)/n$   $\Rightarrow$  residue uncorrelated  
 $\text{DF} = n - \# \text{ of } \beta_i$   $q = \# \text{ of } x_i \text{ in full model}$   
 $r = \# \text{ of } x_i \text{ in reduced}$   
 $F = \frac{(\text{SSE}_r - \text{SSE}_q) / (q-r)}{\text{SSE}_q / df_q}$   $F \geq \text{critical}$  reject  $H_0$

ACF graph Large  $n \rightarrow \hat{\rho}(h)$  normal

Box-Cox  $\lambda^2/|h|$  if  $\lambda \neq 0$ ,  $\log \lambda$  if  $\lambda = 0$   
 Ljung-Box statistics:  $H_0: \rho(h) = 0$   $p < 0.05$ : reject  $H_0$

Sample ACF:  $\hat{\rho}_x(h) = \frac{\sum (x_t - \bar{x})(x_{t+h} - \bar{x})}{\sum (x_t - \bar{x})^2}$   
 Test  $H_0: \rho(1) = 0$ : t-test  $\frac{\hat{\rho}_x(1)}{1/\sqrt{n}}$   $t >$  critical reject  $H_0$

Theory CCF:  $\hat{\rho}_{xy}(h) = \frac{\sum_{t=h+1}^n (x_t - \bar{x})(y_{t-h} - \bar{y})}{\sqrt{\sum_{t=h+1}^n (x_t - \bar{x})^2 \sum_{t=h+1}^n (y_{t-h} - \bar{y})^2}}$   
 Sample CCF:  $\hat{\gamma}_x(0) = \frac{1}{n} \sum (x_t - \bar{x})^2$   $\hat{\gamma}_y(0) = \frac{1}{n} \sum (y_t - \bar{y})^2$   $\hat{\gamma}_{xy}(h) = \frac{1}{n} \sum (x_{t+h} - \bar{x})(y_t - \bar{y})$

Best Linear Predictor  
 given  $x_1, \dots, x_n$ ,  $x_{n+m} = a_0 + \sum a_k x_k$   
 $E((x_{n+m} - \sum a_k x_k) \times x_k) = 0, k = 0, 1, \dots, n, x_0 = 1$  (estimation - true)  $\perp x_k$   
 $E(x_{n+m}) = E(x_{n+m})$  when  $k=0, x_0=1$   
 $x_{n+m} = a_0 + a_1 x_1 + \dots + a_n x_n$

Example:  
 $P(a_1 Y_1 + a_2 Y_2 | Z) = a_1 P(Y_1 | Z) + a_2 P(Y_2 | Z)$   
 BLE satisfy  $E[\sum (Y_t - P(Y_t | Z))] = 0$   
 where  $P(Y_t | Z) = a_1 z + b$   
 $E(Z \cdot Y) - a E(Z^2) - b E(Z)$   
 $E(Z \cdot Y) - a E(Z^2) - (E(Y) - a E(Z)) \cdot E(Z)$   
 $E(Z \cdot Y) - E(Y) \cdot E(Z) + a(E(Z)^2 - a E(Z)^2)$   
 $\text{Cov}(Y, Z) = a V(Z)$   
 get  $a$ , get  $b$ , calculate  $P(Y | Z)$   
 substitute  $Y$  for  $a_1 Y_1 + a_2 Y_2$  in  $P(Y | Z)$

Example:  
 $X_t \sim \text{AR}(1)$ , given  $X_1, X_2$  find BLE of  $X_3$   
 BLE is  $Y = a X_1 + b X_2$  satisfies  $E(X_3(X_1 - Y)) = 0$   
 and  $E(X_3(X_2 - Y)) = 0$  (+)  
 $E(X_t) = \phi E(X_{t-1}) \Rightarrow \mu = E(X) = 0$   
 $\text{AR}(2): \gamma(h) = \sigma_w^2 \frac{\phi^{|h|}}{1 - \phi^2}$   
 solve (+):  $\frac{\phi}{1 - \phi^2} - \frac{a}{1 - \phi^2} - \frac{b \phi}{1 - \phi^2} = 0$ ,  $\frac{\phi}{1 - \phi^2} - \frac{a \phi^2}{1 - \phi^2} - \frac{b}{1 - \phi^2} = 0$   
 get  $a = \phi - \phi^3 b$   
 substitute into 2nd:  $b = \frac{\phi}{1 - \phi^2}$ ,  $a = \frac{\phi}{1 - \phi^2}$   
 back to  $Y$  get  $Y = \frac{\phi}{1 - \phi^2} (X_1 + X_2)$

Yule-Walker equation (for  $\text{AR}(p)$  only)  
 $\sigma_w^2 = \gamma(0) - \phi_1 \gamma(1) - \dots - \phi_p \gamma(p)$   
 $\gamma(h) = \phi_1 \gamma(h-1) + \dots + \phi_p \gamma(h-p), h = 1, 2, \dots, p$

$$\Phi = \Gamma_p^{-1} \hat{\gamma}_p, \hat{\sigma}_w^2 = \hat{\gamma}(0) - \hat{\gamma}_p^T \Gamma_p^{-1} \hat{\gamma}_p \quad \text{or} \quad \Phi = \hat{R}_p^{-1} \hat{r}_p, \hat{\sigma}_w^2 = \hat{\gamma}(0) [1 - \hat{r}_p^T \hat{R}_p^{-1} \hat{r}_p]$$

$$\begin{pmatrix} \phi_1 \\ \phi_2 \\ \vdots \\ \phi_p \end{pmatrix} = \begin{pmatrix} \gamma(0) & \gamma(1) & \dots & \gamma(p-1) \\ \gamma(1) & \gamma(0) & \dots & \gamma(p-2) \\ \vdots & \vdots & \ddots & \vdots \\ \gamma(p-1) & \gamma(p-2) & \dots & \gamma(0) \end{pmatrix}^{-1} \begin{pmatrix} \gamma(1) \\ \gamma(2) \\ \vdots \\ \gamma(p) \end{pmatrix}$$

$$\begin{pmatrix} \phi_1 \\ \phi_2 \\ \vdots \\ \phi_p \end{pmatrix} = \begin{pmatrix} \rho(1) & \rho(2) & \dots & \rho(p-1) \\ \rho(2) & \rho(1) & \dots & \rho(p-2) \\ \vdots & \vdots & \ddots & \vdots \\ \rho(p-1) & \rho(p-2) & \dots & \rho(1) \end{pmatrix}^{-1} \begin{pmatrix} \rho(1) \\ \rho(2) \\ \vdots \\ \rho(p) \end{pmatrix}$$

$$\sigma_w^2 = \hat{\gamma}(0) - (\hat{\gamma}(1) \dots \hat{\gamma}(p)) \cdot \begin{pmatrix} \phi_1 \\ \phi_2 \\ \vdots \\ \phi_p \end{pmatrix} \quad \sigma_w^2 = \hat{\gamma}(0) \cdot [1 - (\rho(1) \dots \rho(p)) \cdot \begin{pmatrix} \phi_1 \\ \phi_2 \\ \vdots \\ \phi_p \end{pmatrix}]$$

Large Sample Asymptotic:  $V(\hat{\phi}) = \frac{\sigma^2 \Gamma_p^{-1}}{n}$   $\frac{\sigma^2 R_p^{-1}}{n \cdot \hat{\gamma}(0)}$  95% CI:  $\hat{\phi}_i \pm 1.96 \cdot \text{se}(\hat{\phi}_i)$   
 $\Phi_{n+m} \sim \mathcal{N}(0, \frac{1}{n})$

Prediction Interval for  $x_{n+m}$

$$x_{n+m} \pm 1.28 \sqrt{\hat{\sigma}_{n+m}^2}$$

$$\begin{cases} \psi_k = \sum_{j=1}^k \phi_j \psi_{k-j} & k < p \\ \psi_k = \sum_{j=1}^p \phi_j \psi_{k-j} & k \geq p \end{cases}$$

AR(2) prediction  
 $x_{n+1}^* = \phi_1 x_n + \phi_2 x_{n-1}$   
 $x_{n+2}^* = \phi_1 x_{n+1} + \phi_2 x_n$   
 $\hat{x}_{n+1} = \phi_1 x_n + \phi_2 x_{n-1}$

(Spectral Density -  $\sum_{h=-\infty}^{\infty} \gamma(h) \exp(-2\pi i w h)$   $-\infty < w < \infty$   
 Normalized SD -  $\sum_{h=-\infty}^{\infty} \rho(h) \exp(-2\pi i w h)$ )

BLE:  $E(x_{n+m} | x_1, \dots, x_n)$   
 $E(w_t | x_1, \dots, x_n) = \begin{cases} 0 & t > n \\ w_t & t \leq n \end{cases}$   
 Example: given  $\text{AR}(1)$   $x_t = c + \phi x_{t-1} + w_t$   
 show  $E(x_{t+h} | x_1, \dots, x_t) \rightarrow E(x_t) = \frac{c}{1-\phi}$   
 Let  $E(x_t) = E(x_{t-1}) = \dots = \mu$   
 $E(x_t) = c + \phi E(x_{t-1}) + E(w_t) \Rightarrow \mu = \frac{c}{1-\phi}$   
 $x_{t+h} = c + \phi x_{t+h-1} + w_{t+h}$   
 $= c + \phi(c + \phi x_{t+h-2} + w_{t+h-1}) + w_{t+h}$   
 $= c + \phi c + \phi^2 c + \dots + \phi^h c + w_{t+h} + \phi w_{t+h-1} + \dots + \phi^h w_t$   
 $E(x_{t+h}) = c + \phi c + \dots + \phi^h c + 0 + \dots + \phi^h w_t$   
 $(|\phi| < 1) |\phi|^h \rightarrow 0 \quad E(x_{t+h} | x_1, \dots, x_t) = c(1 + \phi + \phi^2 + \dots) = \frac{c}{1-\phi}$

Dickey-Fuller Test for stationarity  
 $H_0: \delta = 0, (\phi = 1)$   $(\Delta x_t = x_t - x_{t-1})$   $p \leq 0.05$  reject  $H_0$   
 3 types:  $\Delta x_t = \delta x_{t-1} + w_t$  no drift / trend  
 $\Delta x_t = a_0 + \delta x_{t-1} + w_t$  drift only  
 $\Delta x_t = a_0 + a_1 t + \delta x_{t-1} + w_t$  drift + trend

Residue Analysis  
 $H_0: \rho_e(h) = 0, H_1: \rho_e(h) \neq 0$  not white noise  
 $\hat{\rho}(h) = \sum_{i=1}^n e_i e_{i-h} / \sum_{i=1}^n e_i^2$

(Box-Pierce Portmanteau -  $Q_m = n \sum_{h=1}^m \hat{\rho}^2(h) \sim \chi_{m-p}^2$   
 Ljung-Box Portmanteau -  $Q_m = n(n+2) \sum_{h=1}^m \hat{\rho}^2(h) / (n-h) \sim \chi_{m-p}^2$   
 reject  $H_0$  if  $Q > \chi^2$ )

Durbin-Levinson Algorithm for PACF  
 $\phi_{nn} = \frac{\rho(n) - \sum_{k=1}^{n-1} \phi_{n-1,k} \rho(n-k)}{1 - \sum_{k=1}^{n-1} \phi_{n-1,k} \rho(k)}$   $n \geq 1$   $\rho_{n+1} = \delta(0) \prod_{j=1}^n (1 - \phi_j^2)$   
 $\phi_{nk} = \phi_{n-1,k} - \phi_{nn} \phi_{n-1, n-k}$   $k = 1, \dots, n-1, n \geq 2$

Shapiro test  $\rightarrow$  normality  $H_0$ : normal,  $p \leq 0.05$  reject

Durbin-Watson Test for autocorrelation  
 $H_0$ : not auto correlated or  $x_t = w_t$   
 $d < d_{L\alpha}$ : reject  
 $d > d_{U\alpha}$ : do not reject  
 otherwise: inconclusive  
 $d = \frac{\sum_{t=2}^n (e_t - e_{t-1})^2}{\sum_{t=1}^n e_t^2}$